Updates to Boyle example and several laws

utp/utp_boyle.thy
@@ -5,16 +5,19 @@ imports utp_theory
 begin
 (*>*)
 
-text {* Boyle's law states that k = p * V is invariant. We here encode this as a simple UTP theory.
-        We first create a record to represent the alphabet of the theory consisting of the three
-        variables k, p and V. *}
+text {* In order to exemplify the use of Isabelle/UTP, we mechanise a simple theory representing
+        Boyle's law. Boyle's law states that for an ideal gas at fixed temperature that pressure @{term p} is inversely 
+        proportional to volume @{term V}, or more formally that for @{term "k = p\<cdot>V"} is invariant, for 
+        constant @{term k}. We here encode this as a simple UTP theory. We first create a record to 
+        represent the alphabet of the theory consisting of the three variables \emph{k}, \emph{p} 
+        and \emph{V}. *}
 
 record alpha_boyle =
   boyle_k :: real
   boyle_p :: real
   boyle_V :: real
 
-text {* For now we have to explicitly cast the fields to UTP variables using the VAR syntactic
+text {* For now we have to explicitly cast the fields to lenses using the VAR syntactic
         transformation function -- in future this will be automated. We also have to
         add the definitional equations for these variables to the simplification set for predicates
         to enable automated proof through our tactics. *}
@@ -25,123 +28,179 @@ definition V :: "real \<Longrightarrow> alpha_boyle" where "V = VAR boyle_V"
 
 declare k_def [upred_defs] and p_def [upred_defs] and V_def [upred_defs]
 
+text {* We also prove that our new lenses are well-behaved and independent of each other. A selection
+        of these properties are shown below. *}
+
 lemma vwb_lens_k [simp]: "vwb_lens k"
   by (unfold_locales, simp_all add: k_def)
-
+(*<*)
 lemma vwb_lens_p [simp]: "vwb_lens p"
   by (unfold_locales, simp_all add: p_def)
 
 lemma vwb_lens_V [simp]: "vwb_lens V"
   by (unfold_locales, simp_all add: V_def)
-
+(*>*)
 lemma boyle_indeps [simp]:
   "k \<bowtie> p" "p \<bowtie> k" "k \<bowtie> V" "V \<bowtie> k" "p \<bowtie> V" "V \<bowtie> p"
   by (simp_all add: k_def p_def V_def lens_indep_def)
-
+(*<*)
 lemma boyle_var_ords [usubst]:
   "k \<prec>\<^sub>v p" "p \<prec>\<^sub>v V"
   by (simp_all add: var_name_ord_def)
+(*>*)
 
+subsection {* Static invariant *} 
 
-text {* Next we state Boyle's law using the healthiness condition B and likewise add it to
-        the UTP predicate definitional equation set. The syntax differs a little from UTP;
-        we try not to override HOL constants and so UTP predicate equality is subscripted.
+text {* We first create a simple UTP theory representing Boyle's laws on a single state, as a static
+        invariant healthiness condition. We state Boyle's law using the function \emph{B}, which recalculates
+        the value of the constant @{term k} based on @{term p} and @{term V}. The syntax differs a 
+        little from UTP; we try not to override HOL constants and so UTP predicate equality is subscripted.
         Moreover to distinguish variables denoting a predicate (like $\phi$) from variables
         denoting UTP variables we have to prepend the latter with an ampersand. *}
 
-definition "B(\<phi>) = ((\<exists> k \<bullet> \<phi>) \<and> (&k =\<^sub>u &p * &V))"
+definition "B(\<phi>) = ((\<exists> k \<bullet> \<phi>) \<and> (&k =\<^sub>u &p\<cdot>&V))"
+(*<*) 
 declare B_def [upred_defs]
-
-definition "D1(P) = (($k =\<^sub>u $p * $V \<Rightarrow> $k\<acute> =\<^sub>u $p\<acute> * $V\<acute>) \<and> P)"
-definition "D2(P) = ($k\<acute> =\<^sub>u $k \<and> P)"
-
-declare D1_def [upred_defs]
-declare D2_def [upred_defs]
-
-definition [upred_defs]: "InitSystem ip iV = \<lceil>B(&p =\<^sub>u \<guillemotleft>ip\<guillemotright> \<and> &V =\<^sub>u \<guillemotleft>iV\<guillemotright>)\<rceil>\<^sub>>"
-definition [upred_defs]: "ChangePressure dp = ((&p + \<guillemotleft>dp\<guillemotright> >\<^sub>u 0)\<^sup>\<top> ;; p := &p + \<guillemotleft>dp\<guillemotright> ;; V := (&k/&p))"
-definition [upred_defs]: "ChangeVolume dV = ((&V + \<guillemotleft>dV\<guillemotright> >\<^sub>u 0)\<^sup>\<top> ;; V := &V + \<guillemotleft>dV\<guillemotright> ;; p := (&k/&V))"
+(*>*)
 
 text {* We can then prove that B is both idempotent and monotone simply by application of
-        the predicate tactic. *}
+        the predicate tactic. Idempotence means that healthy predicates cannot be made
+        more healthy. Monotonicity ensures that image of the healthiness functions forms
+        a complete lattice, which is useful to allow the representation of recursive and
+        iterative constructions with the theory. *}
 
 lemma B_idempotent: "B(B(P)) = B(P)"
   by pred_tac
 
-lemma D1_idempotent: "D1(D1(P)) = D1(P)"
-  by rel_tac
-
-lemma D2_idempotent: "D2(D2(P)) = D2(P)"
-  by rel_tac
-
 lemma B_monotone: "X \<sqsubseteq> Y \<Longrightarrow> B(X) \<sqsubseteq> B(Y)"
   by pred_tac
 
-lemma D1_monotone: "X \<sqsubseteq> Y \<Longrightarrow> D1(X) \<sqsubseteq> D1(Y)"
-  by rel_tac
+text {* We also create some example observations; the first (@{term "\<phi>\<^sub>1"}) satisfies Boyle's law and 
+        the second doesn't (@{term "\<phi>\<^sub>2"}). *}
 
-lemma D2_monotone: "X \<sqsubseteq> Y \<Longrightarrow> D2(X) \<sqsubseteq> D2(Y)"
-  by rel_tac
+definition(*<*)[upred_defs]:(*>*) "\<phi>\<^sub>1 = ((&p =\<^sub>u 10) \<and> (&V =\<^sub>u 5) \<and> (&k =\<^sub>u 50))"
+definition(*<*)[upred_defs]:(*>*) "\<phi>\<^sub>2 = ((&p =\<^sub>u 10) \<and> (&V =\<^sub>u 5) \<and> (&k =\<^sub>u 100))"
 
-text {* We also create some example observations; the first satisfies Boyle's law and the second
-        doesn't. *}
+text {* We first prove an obvious property: that these two predicates are different observations. *}
 
-definition [upred_defs]: "\<phi>\<^sub>1 = ((&p =\<^sub>u 10) \<and> (&V =\<^sub>u 5) \<and> (&k =\<^sub>u 50))"
+lemma \<phi>\<^sub>1_diff_\<phi>\<^sub>2: "\<phi>\<^sub>1 \<noteq> \<phi>\<^sub>2"
+  by (pred_tac, metis select_convs num.distinct(5) numeral_eq_iff semiring_norm(87))
 
-definition [upred_defs]: "\<phi>\<^sub>2 = ((&p =\<^sub>u 10) \<and> (&V =\<^sub>u 5) \<and> (&k =\<^sub>u 100))"
-
-text {* We prove that @{const "\<phi>\<^sub>1"} satisfied by Boyle's law by simplication of its definitional
-        equation and then application of the predicate tactic. *}
+text {* We prove that @{const "\<phi>\<^sub>1"} satisfied by Boyle's law by application of the predicate calculus
+        tactic, \emph{pred-tac}. *}
 
 lemma B_\<phi>\<^sub>1: "\<phi>\<^sub>1 is B"
   by (pred_tac)
 
-text {* We prove that @{const "\<phi>\<^sub>2"} does not satisfy Boyle's law by showing it's in fact equal
-        to @{const "\<phi>\<^sub>1"}. We do this via an automated Isar proof. *}
+text {* We prove that @{const "\<phi>\<^sub>2"} does not satisfy Boyle's law by showing that applying \emph{B} to
+        it results in @{const "\<phi>\<^sub>1"}. We prove this using Isabelle's natural proof language, Isar. *}
 
 lemma B_\<phi>\<^sub>2: "B(\<phi>\<^sub>2) = \<phi>\<^sub>1"
 proof -
-  have "B(\<phi>\<^sub>2) = B((&p =\<^sub>u 10) \<and> (&V =\<^sub>u 5) \<and> (&k =\<^sub>u 100))"
+  have "B(\<phi>\<^sub>2) = B(&p =\<^sub>u 10 \<and> &V =\<^sub>u 5 \<and> &k =\<^sub>u 100)"
     by (simp add: \<phi>\<^sub>2_def) 
-  also have "... = ((\<exists> k \<bullet> (&p =\<^sub>u 10) \<and> (&V =\<^sub>u 5) \<and> (&k =\<^sub>u 100)) \<and> (&k =\<^sub>u &p * &V))"
+  also have "... = ((\<exists> k \<bullet> &p =\<^sub>u 10 \<and> &V =\<^sub>u 5 \<and> &k =\<^sub>u 100) \<and> &k =\<^sub>u &p\<cdot>&V)"
+    by (simp add: B_def)
+  also have "... = (&p =\<^sub>u 10 \<and> &V =\<^sub>u 5 \<and> &k =\<^sub>u &p\<cdot>&V)"
     by pred_tac
-  also have "... = ((&p =\<^sub>u 10) \<and> (&V =\<^sub>u 5) \<and> (&k =\<^sub>u &p * &V))"
-    by pred_tac
-  also have "... = ((&p =\<^sub>u 10) \<and> (&V =\<^sub>u 5) \<and> (&k =\<^sub>u 50))"
+  also have "... = (&p =\<^sub>u 10 \<and> &V =\<^sub>u 5 \<and> &k =\<^sub>u 50)"
     by pred_tac
   also have "... = \<phi>\<^sub>1"
     by (simp add: \<phi>\<^sub>1_def)
   finally show ?thesis .
 qed 
 
-lemma D1_ChangePressure: "D1 (ChangePressure dp) = ChangePressure dp"
+subsection {* Dynamic invariants *}
+
+text {* Next we build a relational theory that allows the pressure and volume to be changed,
+        whilst still respecting Boyle's law. We create two dynamic invariants for this purpose. *}
+
+definition "D1(P) = (($k =\<^sub>u $p\<cdot>$V \<Rightarrow> $k\<acute> =\<^sub>u $p\<acute>\<cdot>$V\<acute>) \<and> P)"
+definition "D2(P) = ($k\<acute> =\<^sub>u $k \<and> P)"
+(*<*)
+declare D1_def [upred_defs]
+declare D2_def [upred_defs]
+(*>*)
+
+text {* @{term "D1"} states that if Boyle's law satisfied in the previous state, then it should
+        be satisfied in the next state. We define this by conjunction of the formal specification 
+        of this property with the predicate. The annotations @{term "$p"} and @{term "$p\<acute>"} refer to
+        relational variables $p$ and $p'$. @{term "D2"} states that the constant @{term k} indeed
+        remains constant throughout the evolution of the system, which is also specified as a conjunctive
+        healthiness condition. As before we demonstrate that @{term D1} and @{term D2} are both idempotent
+        and monotone. *}
+
+lemma D1_idempotent: "D1(D1(P)) = D1(P)" by rel_tac
+lemma D2_idempotent: "D2(D2(P)) = D2(P)" by rel_tac
+
+lemma D1_monotone: "X \<sqsubseteq> Y \<Longrightarrow> D1(X) \<sqsubseteq> D1(Y)" by rel_tac
+lemma D2_monotone: "X \<sqsubseteq> Y \<Longrightarrow> D2(X) \<sqsubseteq> D2(Y)" by rel_tac
+
+text {* Since these properties are relational, we discharge them using our relational calculus tactic
+        \emph{rel-tac}. Next we specify three operations that make up the signature of the theory. *}
+
+definition(*<*)[upred_defs]:(*>*) "InitSys ip iV 
+  = ((\<guillemotleft>ip\<guillemotright> >\<^sub>u 0 \<and> \<guillemotleft>iV\<guillemotright> >\<^sub>u 0)\<^sup>\<top> ;; p,V,k := \<guillemotleft>ip\<guillemotright>,\<guillemotleft>iV\<guillemotright>,(\<guillemotleft>ip\<guillemotright>\<cdot>\<guillemotleft>iV\<guillemotright>))"
+
+definition(*<*)[upred_defs]:(*>*) "ChPres dp 
+  = ((&p + \<guillemotleft>dp\<guillemotright> >\<^sub>u 0)\<^sup>\<top> ;; p := &p + \<guillemotleft>dp\<guillemotright> ;; V := (&k/&p))"
+definition(*<*)[upred_defs]:(*>*) "ChVol dV 
+  = ((&V + \<guillemotleft>dV\<guillemotright> >\<^sub>u 0)\<^sup>\<top> ;; V := &V + \<guillemotleft>dV\<guillemotright> ;; p := (&k/&V))"
+
+text {* @{const InitSys} initialises the system with a given initial pressure ($ip$) and volume ($iV$). 
+        It assumes that both are greater than 0 using the assumption construct @{term "c\<^sup>\<top>"} which equates to @{term II}
+        if @{term c} is true and @{term false} (i.e. errant) otherwise. It then creates a state assignment
+        for $p$ and $V$, uses the @{term B} healthiness condition to make it healthy (by calculating $k$), 
+        and finally turns the predicate into a postcondition using the @{term "\<lceil>P\<rceil>\<^sub>>"} function.
+
+        @{const ChPres} raises or lowers the pressure based on an input \emph{dp}. It assumes
+        that the resulting pressure change would not result in a zero or negative pressure, 
+        i.e. $p + dp > 0$. It assigns the updated value to $p$ and recalculates $V$ using the original
+        value of $k$. @{const ChVol} is similar but updates the volume.
+ *}
+
+lemma D1_InitSystem: "D1 (InitSys ip iV) = InitSys ip iV"
   by rel_tac
+
+text {* @{const InitSys} is @{const D1}, since it establishes the invariant for the system. However,
+  it is not @{const D2} since it sets the global value of $k$ and thus can change its value. We can
+  however show that the both @{const ChPres} and @{const ChVol} are both healthy relations. *}
+
+lemma D1: "D1 (ChPres dp) = ChPres dp" and "D1 (ChVol dV) = ChVol dV"
+  by (rel_tac, rel_tac)
   
-lemma D2_ChangePressure: "D2 (ChangePressure dp) = ChangePressure dp"
-  by rel_tac
+lemma D2: "D2 (ChPres dp) = ChPres dp" and "D2 (ChVol dV) = ChVol dV"
+  by (rel_tac, rel_tac)
 
-lemma D1_ChangeVolume: "D1 (ChangeVolume dV) = ChangeVolume dV"
-  by rel_tac
+text {* Finally we show a calculation a simple animation of Boyle's law, where the initial pressure
+  and volume are set to 10 and 4, respectively, and then the pressure is lowered by 2. *} 
 
-lemma D2_ChangeVolume: "D2 (ChangeVolume dV) = ChangeVolume dV"
-  by rel_tac
-
-lemma ChangePressure_example: "(InitSystem 10 5 ;; ChangePressure (-5)) = p,V,k := 5,10,50"
+lemma ChPres_example: 
+  "(InitSys 10 4 ;; ChPres (-2)) = p,V,k := 8,5,40"
 proof -
-  have "InitSystem 10 5 = p,V,k := 10,5,50"
+  -- {* @{const InitSys} yields an assignment to the three variables *}
+  have "InitSys 10 4 = p,V,k := 10,4,40"
     by (rel_tac)
-  hence "(InitSystem 10 5 ;; ChangePressure (-5)) = (ChangePressure (-5))\<lbrakk>10,5,50/$p,$V,$k\<rbrakk>"
+  -- {* This assignment becomes a substitution *}
+  hence "(InitSys 10 4 ;; ChPres (-2)) 
+          = (ChPres (-2))\<lbrakk>10,4,40/$p,$V,$k\<rbrakk>"
     by (simp add: assigns_r_comp alpha)
-  also have "... = ((&p - 5 >\<^sub>u 0)\<^sup>\<top>\<lbrakk>10,5,50/$p,$V,$k\<rbrakk> ;; p := &p - 5 ;; V := &k / &p)"
-    by (simp add: ChangePressure_def lit_num_simps usubst unrest)
-  also have "... = ((\<langle>[p \<mapsto>\<^sub>s 10, V \<mapsto>\<^sub>s 5, k \<mapsto>\<^sub>s 50]\<rangle>\<^sub>a \<triangleleft> (5 :\<^sub>u real) >\<^sub>u 0 \<triangleright> false) ;; p := &p - 5 ;; V := &k / &p)"
+  -- {* Unfold definition of @{const ChPres} *}
+  also have "... = ((&p - 2 >\<^sub>u 0)\<^sup>\<top>\<lbrakk>10,4,40/$p,$V,$k\<rbrakk>
+                        ;; p := &p - 2 ;; V := &k / &p)"
+    by (simp add: ChPres_def lit_num_simps usubst unrest)
+  -- {* Unfold definition of assumption *}
+  also have "... = ((p,V,k := 10,4,40 \<triangleleft> (8 :\<^sub>u real) >\<^sub>u 0 \<triangleright> false) 
+                        ;; p := &p - 2 ;; V := &k / &p)"
     by (simp add: rassume_def usubst alpha unrest)
-  also have "... = (p,V,k := 10,5,50 ;; p := &p - 5 ;; V := &k / &p)"
+  -- {* @{term "8 > 0"} is true; simplify conditional  *}
+  also have "... = (p,V,k := 10,4,40 ;; p := &p - 2 ;; V := &k / &p)"
     by rel_tac
-  also have "... = p,V,k := 5,10,50"
+  -- {* Application of both assignments *}
+  also have "... = p,V,k := 8,5,40"
     by rel_tac
   finally show ?thesis .
 qed
-
-
+(*<*)
 end
+(*>*)
