utp/utp.thy
@@ -14,6 +14,7 @@ theory utp
     utp_wp
     utp_procedure
     utp_theory
+    utp_boyle
     utp_designs
     utp_concurrency
     utp_reactive
